src/dafny/beacon/StateTransition.dfy
@@ -34,17 +34,7 @@ module StateTransition {
     import opened Validators
     import opened Helpers
 
-    /**
-     *  Compute Root/Hash/Bytes32 for different types.
-     *  
-     *  @todo   Use the hash_tree_root from Merkle?.
-     *  @note   The property of hash_tree_root below is enough for 
-     *          proving some invariants. So we may use a module refinement
-     *          to integrate the actual hash_tree_root from Merkle module.
-     */
-    function method hash_tree_root<T(==)>(t : T) : Bytes32 
-        ensures hash_tree_root(t) != DEFAULT_BYTES32
-
+    
     /** 
      *  The Beacon state type.
      *
@@ -429,7 +419,7 @@ module StateTransition {
             decreases |bb.deposits| - i
             invariant s.eth1_deposit_index as int + i <  0x10000000000000000 
             invariant i <= |bb.deposits|
-            invariant s' == s.(eth1_deposit_index := s.eth1_deposit_index as int + i) ;  
+            invariant s' == s.(eth1_deposit_index := (s.eth1_deposit_index as int + i) as uint64) ;  
         {
             s':= process_deposit(s', bb.deposits[i]);
             i := i + 1;
